Launchbury/CoCallCardinality.thy
@@ -28,9 +28,9 @@ next
       hence "one_call_in_path x (x # xs)" by simp
       with Cons show False by simp
     qed
-    with `set xs \<subseteq> ccNeighbors {x'} G`
-    have "x \<in> ccNeighbors {x} G" by auto
-    thus ?thesis by (metis ccNeighbors_ccManyCalls)
+    with `set xs \<subseteq> ccNeighbors x' G`
+    have "x \<in> ccNeighbors x G" by auto
+    thus ?thesis by simp
   qed
 qed
 
@@ -45,7 +45,7 @@ locale CoCallCardinality = CoCallAnalysis + CoCallAnalyisHeap + CorrectArityAnal
   assumes ccHeap_Exp: "ccExp e\<cdot>a \<sqsubseteq> ccHeap \<Delta> e\<cdot>a"
   assumes ccHeap_Heap: "map_of \<Delta> x = Some e' \<Longrightarrow> (Aheap \<Delta> e\<cdot>a) x= up\<cdot>a' \<Longrightarrow> ccExp e'\<cdot>a' \<sqsubseteq> ccHeap \<Delta> e\<cdot>a"
   assumes ccHeap_Extra_Edges:
-    "map_of \<Delta> x = Some e' \<Longrightarrow> (Aheap \<Delta> e\<cdot>a) x = up\<cdot>a' \<Longrightarrow> ccProd (fv e') (ccNeighbors {x} (ccHeap \<Delta> e\<cdot>a) - {x} \<inter> thunks \<Delta>) \<sqsubseteq> ccHeap \<Delta> e\<cdot>a"
+    "map_of \<Delta> x = Some e' \<Longrightarrow> (Aheap \<Delta> e\<cdot>a) x = up\<cdot>a' \<Longrightarrow> ccProd (fv e') (ccNeighbors x (ccHeap \<Delta> e\<cdot>a) - {x} \<inter> thunks \<Delta>) \<sqsubseteq> ccHeap \<Delta> e\<cdot>a"
 
   assumes aHeap_thunks_rec: " \<not> nonrec \<Gamma> \<Longrightarrow> x \<in> thunks \<Gamma> \<Longrightarrow> x \<in> edom (Aheap \<Gamma> e\<cdot>a) \<Longrightarrow> (Aheap \<Gamma> e\<cdot>a) x = up\<cdot>0"
   assumes aHeap_thunks_nonrec: "nonrec \<Gamma> \<Longrightarrow> x \<in> thunks \<Gamma> \<Longrightarrow> x \<in> ccManyCalls (ccExp e\<cdot>a) \<Longrightarrow> (Aheap \<Gamma> e\<cdot>a) x = up\<cdot>0"
@@ -294,7 +294,7 @@ next
           by (auto simp add: Fexp.AnalBinds_lookup Fexp_simp  intro: below_trans[OF cc_restr_below_arg])
       qed
 
-      show "ccProd (ccNeighbors {x} (ccHeap \<Delta> e\<cdot>a)- {x} \<inter> thunks \<Delta>) (carrier ((Fexp.AnalBinds  \<Delta>\<cdot>(Aheap \<Delta> e\<cdot>a)) x)) \<sqsubseteq> ccHeap \<Delta> e\<cdot>a"
+      show "ccProd (ccNeighbors x (ccHeap \<Delta> e\<cdot>a)- {x} \<inter> thunks \<Delta>) (carrier ((Fexp.AnalBinds  \<Delta>\<cdot>(Aheap \<Delta> e\<cdot>a)) x)) \<sqsubseteq> ccHeap \<Delta> e\<cdot>a"
       proof(cases "(Aheap \<Delta> e\<cdot>a) x")
         case bottom thus ?thesis using e' by (simp add: Fexp.AnalBinds_lookup)
       next
@@ -303,7 +303,7 @@ next
           using up e' by (auto simp add: Fexp.AnalBinds_lookup carrier_Fexp dest!: set_mp[OF Aexp_edom])
         
         from e' up
-        have "ccProd (fv e') (ccNeighbors {x} (ccHeap \<Delta> e\<cdot>a) - {x} \<inter> thunks \<Delta>) \<sqsubseteq> ccHeap \<Delta> e\<cdot>a"
+        have "ccProd (fv e') (ccNeighbors x (ccHeap \<Delta> e\<cdot>a) - {x} \<inter> thunks \<Delta>) \<sqsubseteq> ccHeap \<Delta> e\<cdot>a"
           by (rule ccHeap_Extra_Edges)
         then
         show ?thesis using e'
